Nearly complete General Model with full substitutions

src/named/GeneralModel.v
@@ -37,7 +37,18 @@ Definition meta_subst := named_list exp.
 
 Definition term := meta_subst -> exp.
 
-Definition sort := Type.
+Definition sort := meta_subst -> Type.
+
+Definition ctx : Type := named_list sort.
+
+  Definition eq_sort (_ : ctx) (s1 s2 : sort) :=
+    s1 = s2.
+
+  Definition wf_sort (_ : ctx) (_ : sort) := True.
+
+  Definition eq_term (c : ctx) (_ : sort) (t1 t2 : term) :=
+    (* TODO: check if this is the right way around *)
+    forall (s : named_list exp), NoDup (map fst s) -> incl (map fst c) (map fst s) -> t1 s = t2 s.
 
 Notation Substable0 := (Substable0 V).
 Notation Substable := (@Substable V).
@@ -49,25 +60,56 @@ Definition inj_var (v : V) : term :=
 
 Definition apply_subst (l : named_list term) (t : term) : term :=
   fun (ms' : meta_subst) =>
-    t ((named_map (fun x => x ms') l) ++ ms').
+    t ((named_map (fun x => x ms') l)).
 
 Definition id_args {B} (c : named_list B) :=
   map inj_var (map fst c).
 
 Notation id_subst c := (with_names_from c (id_args c)).
 
-Definition id_substable {B} (e : term) :=
-  forall (c : named_list B), e = apply_subst (id_subst c) e.
+(* TODO change to eq_term *)
+Definition eq_term0 args (e1 e2 : term) :=
+  forall ms, map fst ms = args -> e1 ms = e2 ms.
 
+Lemma eq_term0_refl : forall args e1, eq_term0 args e1 e1.
+Proof.
+  unfold eq_term0.
+  trivial.
+Qed.
+
+Lemma eq_term0_trans : forall args e1 e2 e3, eq_term0 args e1 e2 -> eq_term0 args e2 e3 -> eq_term0 args e1 e3.
+Proof.
+  unfold eq_term0.
+  intros.
+  rewrite H; trivial.
+  apply H0; trivial.
+Qed.
+
+Lemma eq_term0_comm : forall args e1 e2, eq_term0 args e1 e2 -> eq_term0 args e2 e1.
+Proof.
+  unfold eq_term0.
+  symmetry.
+  apply H; trivial.
+Qed.
+
+
+(* TODO make this simpler? *)
 Definition ws_term args (e : term) :=
-    (forall s, map fst s = args ->
-         forall s', (forall arg, In arg args -> named_list_lookup default s' arg = named_list_lookup default s arg) ->
-           e s' = e s)
-  /\ forall B, id_substable (B:=B) e.
+  NoDup args /\
+  forall s, map fst s = args -> forall s', NoDup (map fst s') -> incl s s' -> e s' = e s.
+
+Definition id_substable {B} (e : term) :=
+  forall (c : named_list B),
+    ws_term (map fst c) e
+    -> forall args, ws_term args e
+              -> eq_term0 args e (apply_subst (id_subst c) e).
+
+Definition wf_term (c : ctx) t (_ : sort) := ws_term (map fst c) t.
 
 Instance substable_term : Substable0 term :=
   {
     inj_var := inj_var;
+    eq_term0 := eq_term0;
     apply_subst0 := apply_subst;
     well_scoped0 := ws_term
   }.
@@ -75,27 +117,19 @@ Instance substable_term : Substable0 term :=
 Instance substable_sort : Substable term sort :=
   {
     apply_subst := fun _ B => B;
+    eq_term := fun _ => eq;
     well_scoped := fun _ _ => True
   }.
-
-Definition ctx : Type := named_list sort.
-
-  Definition eq_sort (_ : ctx) (s1 s2 : sort) :=
-    s1 = s2.
-
-  Definition wf_sort (_ : ctx) (_ : sort) := True.
-
-  Definition eq_term (_ : ctx) (_ : sort) (t1 t2 : term) :=
-    forall (s : named_list exp), t1 s = t2 s.
-
-  Definition wf_term (c : ctx) t (_ : sort) := ws_term (map fst c) t.
 
 Notation Model := (@Model V term sort).
 
 #[export] Instance model : Model := mut_mod eq_sort eq_term wf_sort wf_term.
 
 Ltac unfold_all :=
-  repeat (unfold apply_subst, inj_var, subst_lookup, pair_map_snd, wf_term, Substable.apply_subst in *; simpl in *).
+  repeat (
+      unfold ws_term, apply_subst, inj_var, subst_lookup, pair_map_snd,
+      wf_term, Substable.apply_subst, eq_term0 in *;
+      simpl in *).
 
 Ltac cases x :=
   case_eq x; intros;
@@ -156,32 +190,227 @@ Ltac model_crush :=
      | [|- _ :: _ = _ :: _] => apply invert_eq_cons_cons
      | [|- (_, _) = (_, _)] => apply pair_equal_spec
      | [H : _ :: _ = _ :: _ |- _] => apply invert_eq_cons_cons in H
+     | [H : NoDup (_ :: ?a) |- NoDup ?a ] => apply NoDup_cons_iff in H
      | [H : (_, _) = (_, _) |- _] => apply pair_equal_spec in H
-     | [H : _ = _ |- _] => try rewrite H
      | [H : ws_term _ ?a |- ws_term _ ?a] => apply H
      | [ |- map fst (named_map _ _) = map fst _] => symmetry
+     | [ |- incl [] _ ] => apply incl_nil_l
      | [ |- map fst _ = map fst (named_map _ _)] => repeat apply named_map_fst'; trivial
+     | [ H : eqb _ _ = false |- _ ] => try apply eqb_neq in H
+     | [ H : eqb _ _ = true |- _ ] => try apply eqb_eq in H
+     | [ |- eqb _ _ = false ] => try apply eqb_neq
+     | [ |- eqb _ _ = true ] => try apply eqb_eq
+     | [H : ?a <> ?a |- _] => contradiction
+     | [H : ?a = _ |- _] => rewrite H in *
      | _ => idtac
      end;
      try rewrite <- named_map_fst;
+     try rewrite map_fst_with_names_from;
+     try rewrite map_length;
      if_refl
     ).
+
+  Fixpoint inb {A} `{Eqb A} (a : A) l :=
+    match l with
+    | [] => false
+    | e :: l' => orb (eqb a e) (inb a l')
+    end.
+
+  Lemma inb_in {A} `{Eqb A} : forall (a : A) l, inb a l = true -> In a l.
+  Proof.
+    intros.
+    induction l.
+    contradict H0; simpl; auto.
+    simpl in *.
+    cases (eqb a0 a).
+    left; trivial.
+    right; destruct H0.
+    apply not_eq_sym in H1.
+    apply eqb_neq in H1.
+    rewrite H1 in IHl.
+    simpl in IHl.
+    apply IHl; trivial.
+  Qed.
+
+  Lemma not_or : forall A B, ~ A -> ~B -> ~ (A \/ B).
+  Proof.
+    intros.
+    apply neg_false; constructor; intros; try contradiction.
+    destruct H1; contradict H1; assumption.
+  Qed.
+
+  Lemma inb_not_in {A} `{Eqb A} : forall (a : A) l, inb a l = false -> (~ In a l).
+  Proof.
+    intros.
+    induction l.
+    - apply in_nil.
+    - model_crush; apply Bool.orb_false_iff in H0; destruct H0.
+      apply not_or.
+      apply eqb_neq in H0; auto.
+      apply (IHl H1).
+  Qed.
+
+  Fixpoint merge_named_lists {A} (l1 l2 : named_list A) :=
+    match l1 with
+    | [] => l2
+    | (v, e) :: l1' =>
+        if (inb v (map fst l2))
+        then merge_named_lists l1' l2
+        else (v, e) :: merge_named_lists l1' l2
+    end.
+
+  Lemma merge_named_lists_in_l2 {A} (l1 l2 : named_list A) x :
+    In x l2 -> In x (merge_named_lists l1 l2).
+  Proof.
+    induction l1; model_crush.
+    case (inb v0 (map fst l2)); try apply in_cons; try apply H.
+  Qed.
+
+  Lemma merge_named_lists_incl {A} (l1 l2 : named_list A) : 
+    incl l2 (merge_named_lists l1 l2).
+  Proof.
+    induction l1; model_crush; try apply incl_refl.
+    case (inb v (map fst l2)).
+    - apply IHl1.
+    - apply incl_tl.
+      apply IHl1.
+  Qed.
+
+  Lemma named_list_lookup_in : forall l v e, In v (map fst l) -> named_list_lookup default l v = e -> In (v, e) l.
+  Proof.
+    induction l; model_crush.
+    left; rewrite <- H0; model_crush.
+    cases (eqb v v0).
+    left; rewrite <- H0; model_crush.
+    right; apply IHl; try rewrite <- H0; model_crush.
+  Qed.
+
+
+  Lemma merge_named_lists_incl_l (l1 l2 : named_list exp) :
+    NoDup (map fst l1) ->
+    (forall v, In v (map fst l1) -> In v (map fst l2) -> named_list_lookup default l1 v = named_list_lookup default l2 v) ->
+    incl l1 (merge_named_lists l1 l2).
+  Proof.
+    induction l1; model_crush.
+    specialize (H0 v (or_introl eq_refl)) as H1.
+    assert (eqb v v = true) by apply eqb_refl.
+    rewrite H2 in H1; clear H2.
+    apply incl_cons; cases (inb v (map fst l2)); model_crush.
+    - apply inb_in in H2.
+      specialize (H1 H2).
+      apply merge_named_lists_in_l2.
+      apply named_list_lookup_in; model_crush.
+    - apply IHl1; model_crush.
+      specialize (H0 v0).
+      case_eq (eqb v0 v); intros; rewrite H5 in *.
+      + apply NoDup_cons_iff in H.
+        destruct H.
+        apply eqb_eq in H5.
+        rewrite H5 in *.
+        apply H in H3; contradiction.
+      + apply H0; model_crush.
+        right; apply H3.
+    - left; trivial.
+    - apply incl_tl; apply IHl1; model_crush.
+      specialize (H0 v0).
+      case_eq (eqb v0 v); intros; rewrite H5 in *.
+      + apply NoDup_cons_iff in H.
+        destruct H.
+        apply eqb_eq in H5.
+        rewrite H5 in *.
+        apply H in H3; contradiction.
+      + apply H0; model_crush.
+        right; apply H3.
+Qed.
+
+  Lemma merge_named_lists_not_in {A} : forall (l1 l2 : named_list A) a,
+    ~ In a l1 -> ~ In a l2 -> ~ In a (merge_named_lists l1 l2).
+  Proof.
+    intros.
+    induction l1; model_crush.
+    apply Decidable.not_or in H; destruct H.
+    apply IHl1 in H1.
+    cases (inb v0 (map fst l2)); model_crush.
+    apply not_or; auto.
+  Qed.
+
+  Lemma merge_named_lists_not_in_fst {A} : forall (l1 l2 : named_list A) a,
+    ~ In a (map fst l1) -> ~ In a (map fst l2) -> ~ In a (map fst (merge_named_lists l1 l2)).
+  Proof.
+    intros.
+    induction l1; model_crush.
+    apply Decidable.not_or in H; destruct H.
+    apply IHl1 in H1.
+    cases (inb v (map fst l2)); model_crush.
+    apply not_or; auto.
+Qed.
+
+  Lemma NoDup_merged_lists {A} : forall (l1 l2 : named_list A),
+    NoDup (map fst l1) -> NoDup (map fst l2) -> NoDup (map fst (merge_named_lists l1 l2)).
+  Proof.
+    intros.
+    induction l1; model_crush; apply NoDup_cons_iff in H; destruct H; apply IHl1 in H1.
+    cases (inb v (map fst l2)); model_crush.
+    apply NoDup_cons.
+    apply inb_not_in in H2.
+    apply merge_named_lists_not_in_fst; assumption.
+    assumption.
+  Qed.
+
+  Lemma in_lookup : forall v ms, In v (map fst ms) -> In (v, named_list_lookup default ms v) ms.
+  Proof.
+    intros.
+    induction ms; model_crush.
+    left; model_crush; destruct H0; trivial.
+    cases (eqb v v0).
+    left; trivial.
+    right; trivial.
+Qed.
+
+  Lemma id_substable_pf {B : Type}: forall e,
+    id_substable (B:=B) e.
+  Proof.
+    unfold id_substable.
+    unfold eq_term0.
+    model_crush.
+    specialize (H3 (named_map (fun x : meta_subst -> exp => x ms) (id_subst c))).
+    specialize (H2 ms H1).
+    rewrite <- H3 with (s' := (merge_named_lists (named_map (fun x => x ms) (id_subst c)) ms)); model_crush.
+    symmetry; apply H2; model_crush.
+    all: unfold id_args; model_crush.
+    apply NoDup_merged_lists; model_crush.
+    apply merge_named_lists_incl; model_crush.
+    apply NoDup_merged_lists; model_crush.
+    clear H3.
+    induction c; model_crush; try apply incl_nil_l.
+    apply List.incl_cons; cases (inb v args).
+    * apply merge_named_lists_in_l2.
+      apply in_lookup.
+      rewrite H1.
+      apply inb_in; trivial.
+    * apply in_eq.
+    * apply IHc.
+      apply NoDup_cons_iff in H.
+      destruct H.
+      trivial.
+    * apply incl_tl.
+      apply IHc.
+      apply NoDup_cons_iff in H.
+      destruct H.
+      trivial.
+Qed.
 
 
   Lemma eqb_eq_eqb : forall (H1 H2 : Eqb V) (x y : V), eqb (Eqb:=H1) x y = eqb (Eqb:=H2) x y.
     Proof.
       intros.
-      case_eq (eqb x y); intros.
-      apply eqb_eq in H.
-      apply eqb_eq.
-      trivial.
-      apply eqb_neq in H.
-      apply eqb_neq.
-      trivial.
+      case_eq (eqb x y); model_crush.
 Qed.
 
   Lemma subst_var : forall (H : Eqb V) (s : named_list term) (x : V),
-      apply_subst s (inj_var x) = subst_lookup s x.
+      In x (map fst s) ->
+      forall args,
+      eq_term0 args (apply_subst s (inj_var x)) (subst_lookup s x).
   Proof.
     model_crush.
     induction s; model_crush.
@@ -191,18 +420,17 @@ Qed.
   Proof.
     model_crush.
     induction l1; model_crush.
-    rewrite H in H0; contradict H0; apply eq_refl.
 Qed.
 
-  Lemma ws_term_append : forall (args : list V) (l1 l2 : named_list exp) (a : term),
-      ws_term args a -> map fst l1 = args -> a (l1 ++ l2) = a l1.
-  Proof.
-    model_crush.
-    apply H; model_crush.
-    apply lookup_found.
-    unfold ws_term in H.
-    rewrite <- H0 in H1; trivial.
-  Qed.
+  (* Lemma ws_term_append : forall (args : list V) (l1 l2 : named_list exp) (a : term), *)
+  (*     ws_term args a -> map fst l1 = args -> a (l1 ++ l2) = a l1. *)
+  (* Proof. *)
+  (*   model_crush. *)
+  (*   apply H; model_crush. *)
+  (*   apply lookup_found. *)
+  (*   unfold ws_term in H. *)
+  (*   rewrite <- H0 in H1; trivial. *)
+  (* Qed. *)
 
   Lemma named_map_cons_eq {A B} : forall l (n : V) (e : A) (f : A -> B),
       named_map f ((n, e) :: l) = (n, f e) :: named_map f l.
@@ -219,7 +447,8 @@ Qed.
 Qed.
 
   Lemma subst_assoc0 : forall (s1 s2 : named_list term) (a : term),
-      ws_term (map fst s2) a -> apply_subst s1 (apply_subst s2 a) = apply_subst (subst_cmp s1 s2) a.
+      ws_term (map fst s2) a -> forall args,
+        eq_term0 args (apply_subst s1 (apply_subst s2 a)) (apply_subst (subst_cmp s1 s2) a).
   Proof.
     model_crush.
     repeat erewrite ws_term_append; model_crush.
@@ -230,13 +459,12 @@ Qed.
   Qed.
 
   Lemma subst_id0 {B} : forall (c : named_list B) (a : term),
-      ws_term (map fst c) a -> apply_subst (id_subst c) a = a.
+      ws_term (map fst c) a -> forall args, ws_term args a -> eq_term0 args (apply_subst (id_subst c) a) a.
   Proof.
     intros.
-    destruct H.
-    unfold id_substable in H0.
-    specialize (H0 B c).
-    auto.
+    pose proof (id_substable_pf (B := B) (e := a) c) as id_sub.
+    apply eq_term0_comm.
+    apply id_sub; model_crush.
 Qed.
 
   Lemma in_fst {A} : forall n (e : A) (l : named_list A), In (n, e) l -> In n (map fst l).
@@ -255,30 +483,14 @@ Qed.
 
   Lemma strengthen_subst0 : forall (s : named_list term) (e a : term) (n : V),
       ws_term (map fst s) a -> fresh n s ->
-      apply_subst ((n, e) :: s) a = apply_subst s a.
+      forall args,
+      eq_term0 args (apply_subst ((n, e) :: s) a) (apply_subst s a).
   Proof.
-    intros.
-    unfold apply_subst.
-    apply functional_extensionality; intros.
-    symmetry; erewrite ws_term_append at 1.
-    remember (fun t => t x) as f.
-    pose proof (named_map_fst s f (A := (meta_subst -> exp))) as nmf.
-    symmetry in nmf.
-    destruct H.
-    specialize (H (named_map f s) nmf (named_map f ((n, e) :: s) ++ x)).
-    symmetry; apply H.
-    intros.
-    unfold fresh in H0.
-    rewrite named_map_cons_eq.
-    case_eq (eqb arg n); intros.
-    apply eqb_eq in H3.
-    rewrite H3 in H2.
-    apply H0 in H2; contradiction.
-    simpl.
-    rewrite H3.
-    apply lookup_found.
-    rewrite nmf; trivial.
-    all: model_crush.
+    model_crush.
+    apply H1; simpl; try rewrite <- named_map_fst in *; simpl; trivial.
+    apply NoDup_cons; assumption.
+    apply incl_tl.
+    apply incl_refl.
 Qed.
 
   Lemma fun_app_eq {A B} : forall (f g : A -> B) (a : A), f = g -> f a = g a.
@@ -286,52 +498,50 @@ Qed.
     model_crush.
   Qed.
 
+  Lemma ws_extend : forall (args : list V) (v : V) (t : term),
+      ~In v args -> ws_term args t -> ws_term (v :: args) t.
+  Proof.
+    unfold ws_term in *.
+    model_crush.
+    apply NoDup_cons; trivial.
+    induction s; model_crush.
+    inversion H2.
+    clear IHs.
+    assert (t s' = t s).
+    apply H1; model_crush.
+    apply incl_cons in H4.
+    model_crush.
+    rewrite H6.
+    symmetry.
+    apply H1; model_crush.
+    apply NoDup_cons; trivial.
+    apply incl_tl.
+    apply incl_refl.
+Qed.
+
   Lemma well_scoped_subst0 : forall (args : list V) (s : named_list term) (a : term),
+      NoDup args ->
       ws_subst args s ->
       ws_term (map fst s) a ->
       ws_term args (apply_subst s a).
   Proof.
     model_crush.
-    constructor; model_crush.
-    + repeat erewrite ws_term_append; model_crush; model_crush.
-      f_equal.
-      clear H0.
-      induction s.
-      trivial.
-      destruct a0.
-      repeat rewrite named_map_cons_eq.
-      destruct H.
-      destruct H0.
-      destruct H0.
-      specialize (H0 s0 H1 s' H2).
-      rewrite H0.
-      rewrite IHs; trivial.
-    + unfold id_substable.
-      model_crush.
-      repeat erewrite ws_term_append; model_crush; model_crush.
-      clear H0.
-      f_equal.
-      induction s.
-      model_crush.
-      unfold ws_subst in H.
-      destruct a0.
-      destruct H.
-      destruct H0.
-      destruct H0.
-      unfold id_substable in H2.
-      specialize (H2 B c).
-      apply fun_app_eq with (a := x) in H2.
-      model_crush.
+    f_equal.
+    clear H2.
+    induction s; model_crush.
+    apply H7; model_crush.
 Qed.
 
 Instance substable_term_ok : Substable0_ok term.
 constructor; intros.
-- apply subst_var.
+- apply subst_var; trivial.
+  admit.
 - apply subst_assoc0; trivial.
-- apply subst_id0; trivial.
+- apply subst_id0; constructor; destruct H, H0; trivial.
 - apply strengthen_subst0; trivial.
 - apply well_scoped_subst0; trivial.
-Qed.
+  admit.
+Admitted.
 
 Instance substable_sort_ok : Substable_ok term sort.
 Proof.
@@ -341,15 +551,21 @@ Qed.
 
 
 
-  Lemma term_subst_id_eq {A} : forall (c : named_list A) n, apply_subst (with_names_from c (map inj_var (map fst c))) (inj_var n) = inj_var n.
-    Proof.
-      model_crush.
-      induction c; model_crush.
+  (* Lemma term_subst_id_eq {A} : forall (c : named_list A) n, apply_subst (with_names_from c (map inj_var (map fst c))) (inj_var n) = inj_var n. *)
+  (*   Proof. *)
+  (*     model_crush. *)
+  (*     induction c; model_crush. *)
+  (* Qed. *)
+
+  Lemma eq_subst_dom_eq_l : forall c c' s1 s2, eq_subst c c' s1 s2 -> map fst c' = map fst s1.
+  Proof.
+    induction 1; model_crush.
   Qed.
 
   Lemma eq_term_subst : forall (c : ctx) (s1 s2 : named_list term)
-                      (c' : ctx) (t : sort) 
+                      (c' : ctx) (t : sort)
                       (e1 e2 : term),
+                    NoDup (map fst c') ->
                     eq_subst c c' s1 s2 ->
                     eq_term c' t e1 e2 ->
                     eq_term c t [/s2 /] e1 [/s1 /] e2 [/s2 /].
@@ -357,71 +573,152 @@ Qed.
       unfold eq_term in *.
       unfold Substable.apply_subst.
       model_crush.
-      rewrite H0.
+      rewrite H1; model_crush.
       f_equal.
-      apply app_inv_tail_iff.
-      induction H; model_crush.
+      clear H1.
+      induction H0; model_crush.
+      unfold eq_term in H1.
+      apply H1; trivial.
+      apply IHeq_subst; trivial.
+      apply NoDup_cons_iff in H; model_crush.
+      all: erewrite <- eq_subst_dom_eq_l; try apply H0; model_crush.
+      apply incl_refl.
+Qed.
+
+  Lemma lookup_found_nodup {A} :
+    forall (c : named_list A) (n : V) (default : A) (a : A),
+      NoDup (map fst c) -> In (n, a) c -> a = named_list_lookup default c n.
+    Proof.
+      model_crush.
+      induction c; model_crush.
+      inversion H.
+      apply in_fst in H0.
+      apply H4 in H0; contradiction.
+      apply IHc; model_crush.
     Qed.
 
+
+  Lemma incl_nodup_eq {A} :
+    forall (l l' : named_list A) (n : V) (a a' : A),
+      incl ((n, a) :: l) ((n, a') :: l') -> NoDup (n :: map fst l') -> a = a'.
+      Proof.
+        intros.
+        induction l; model_crush.
+        unfold incl in H.
+        specialize (H (n, a)).
+        model_crush.
+        assert ((n, a) = (n, a) \/ False) by (left; reflexivity).
+        apply H in H1.
+        model_crush.
+        apply in_fst in H1.
+        inversion H0.
+        apply H4 in H1; contradiction.
+        apply IHl.
+        apply incl_cons in H; destruct H.
+        apply incl_cons in H1; destruct H1.
+        apply incl_cons.
+        constructor; trivial.
+      Qed.
+
+  Lemma in_fst_in {A} : forall (c c' : named_list A) n a,
+      In n (map fst c) -> NoDup (n :: map fst c') -> incl c ((n, a) :: c') -> In (n, a) c.
+  Proof.
+    model_crush.
+    induction c, c'.
+    - model_crush.
+    - model_crush.
+    - specialize (H1 a0); simpl in H1.
+      destruct H1.
+      left; trivial.
+      rewrite <- H1.
+      apply in_eq.
+      contradiction.
+    - model_crush.
+      left; model_crush.
+      eapply incl_nodup_eq.
+      apply H1.
+      apply H0.
+      right; model_crush.
+      apply NoDup_cons_iff in H0; model_crush.
+      apply incl_cons in H1; model_crush.
+  Qed.
+
+  Lemma in_in_fst {A} : forall (c : named_list A) n,
+    In n (map fst c) -> exists a, In (n, a) c.
+  Proof.
+    model_crush.
+    induction c; inversion H.
+    exists (snd a); model_crush; left; trivial.
+    apply IHc in H0.
+    simpl.
+    case H0.
+    intros.
+    exists (x).
+    right.
+    apply H1.
+  Qed.
+
+  Lemma named_list_lookup_incl : forall s s' n,
+      NoDup (map fst s) -> NoDup (map fst s') -> In n (map fst s) -> incl s s' -> named_list_lookup default s n = named_list_lookup default s' n.
+  Proof.
+    model_crush.
+    specialize (in_in_fst s n H1); intros.
+    case H3; intros.
+    erewrite <- lookup_found_nodup with (c := s).
+    apply lookup_found_nodup.
+    1, 3: trivial.
+    2: apply H4.
+    apply (H2 (n, x) H4).
+Qed.
+
   Lemma wf_term_var : forall (c : list V) (n : V),
-                  In n c -> ws_term c (inj_var n).
+      NoDup c -> In n c -> ws_term c (inj_var n).
   Proof.
     model_crush.
-    constructor; model_crush.
-    - apply H1; trivial.
-    - unfold id_substable; model_crush.
-      induction c0; model_crush.
-  Qed.
+    rewrite <- H1 in *.
+    clear H1.
+    symmetry.
+    apply named_list_lookup_incl; trivial.
+Qed.
 
-  Lemma wf_subst_same_name : forall c' s c, wf_subst c' s c -> map fst c = map fst s.
+      Print wf_subst.
+      Inductive wf_subst' : list V -> subst -> Prop :=
+      | wf_subst_nil' : forall c, wf_subst' c []
+      | wf_subst_cons' : forall c s name e, wf_subst' c s ->
+                         ws_term c e ->
+                         wf_subst' c ((name, e) :: s).
+
+  Lemma wf_subst_wf_subst' : forall c s c', wf_subst c s c' -> wf_subst' (map fst c) s.
   Proof.
     model_crush.
-    induction H; model_crush.
+    induction H.
+    apply wf_subst_nil'.
+    apply wf_subst_cons'; model_crush.
   Qed.
-
 
   Lemma wf_term_subst_monotonicity : forall (c : ctx) (e : term) (t : sort),
       wf_term c e t ->
       wf_ctx c ->
       forall (c'' : ctx) (s : named_list term),
+        NoDup (map fst c'') ->
         wf_subst c'' s c ->
         wf_term c'' e[/s/] t [/s/].
   Proof.
-    constructor; unfold Substable.apply_subst; model_crush.
-    + repeat erewrite ws_term_append; model_crush; model_crush.
-      clear H.
-      f_equal.
-      induction H1.
-      trivial.
-      inversion H0.
-      simpl.
-      rewrite IHwf_subst.
-      inversion H.
-      specialize (H10 s0 H2 s' H3).
-      rewrite H10.
-      trivial.
-      trivial.
-      all: erewrite <- wf_subst_same_name; eauto.
-    + unfold id_substable.
-      model_crush.
-      apply wf_subst_same_name in H1 as Hs.
-      repeat erewrite ws_term_append; model_crush; model_crush.
-      f_equal.
-      clear H.
-      induction H1; trivial.
-      simpl.
-      inversion H0.
-      rewrite IHwf_subst; trivial.
-      inversion H.
-      unfold id_substable in H9.
-      specialize (H9 B c0).
-      apply fun_app_eq with (a := x) in H9.
-      rewrite H9.
-      trivial.
-      apply wf_subst_same_name in H1.
-      trivial.
-      all: erewrite <- wf_subst_same_name; eauto.
-Qed.
+    model_crush.
+    f_equal.
+    clear H0.
+    Print wf_subst.
+    apply wf_subst_wf_subst' in H2.
+    induction s; model_crush.
+    inversion H2; model_crush.
+    2: {
+      apply IHs.
+      inversion H2.
+      assumption.
+    }
+    unfold ws_term in H10; model_crush.
+    apply H12; trivial.
+  Qed.
 
   Instance model_ok : Model_ok model.
   Proof.
@@ -432,18 +729,19 @@ Qed.
     + unfold eq_sort in *; inversion H; inversion H0; trivial.
     + unfold eq_sort in *; symmetry; trivial.
     + apply eq_term_subst with (c' := c'); trivial.
+      admit.
     + unfold eq_term in *; trivial.
-    + unfold eq_term in *; intros; rewrite H; trivial.
-    + unfold eq_term in *; symmetry; trivial.
-    + apply wf_term_var; trivial; eapply in_fst; apply H.
+    + unfold eq_term in *; intros; rewrite H; trivial; apply H0; model_crush.
+    + unfold eq_term in *; symmetry; trivial; apply H; model_crush.
+    + apply wf_term_var; trivial.
+      admit.
+      eapply in_fst; apply H.
     + apply wf_term_subst_monotonicity with (c := c); trivial.
-Qed.
+      admit.
+Admitted.
 
 Class Model_from_exp :=
   {
     subst_term := substable_term;
     subst_sort := substable_sort
-  }.
-
-
-End WithExp.
+}.
