src/named/NatLang.v
@@ -1,0 +1,75 @@
+Set Implicit Arguments.
+Set Bullet Behavior "Strict Subproofs".
+
+Require Import String List.
+Import ListNotations.
+Open Scope string.
+Open Scope list.
+From Utils Require Import Utils.
+From Named Require Import Core Elab
+     SimpleVSubst SimpleUnit Matches.
+Import Core.Notations.
+
+Require Coq.derive.Derive.
+
+Definition nat_lang_def : lang :=
+  {[l
+  [s|
+      -----------------------------------------------
+      #"natural" srt
+  ];
+  [:|  
+       -----------------------------------------------
+       #"0" : #"natural"
+  ];
+  [:|  "n": #"natural"
+       -----------------------------------------------
+       #"1+" "n" : #"natural"
+  ];
+  [:|
+       "a" : #"natural",
+       "b" : #"natural" 
+       -----------------------------------------------
+       #"plus" "a" "b" : #"natural"
+  ];
+  [:=
+       "a" : #"natural"
+       ----------------------------------------------- ("plus_0")
+       #"plus" "a" #"0" = "a" : #"natural"
+  ];
+  [:=
+       "a" : #"natural",
+       "b" : #"natural"
+       ----------------------------------------------- ("plus_1+")
+       #"plus" "a" (#"1+" "b") = #"plus" (#"1+" "a") "b" : #"natural"
+  ]
+
+
+  (* [s|  "n": #"natural", "m": #"natural" *)
+  (*      ----------------------------------------------- *)
+  (*      #"neq" "n" "m" srt *)
+  (* ]; *)
+  (* [:|  "n": #"natural" *)
+  (*      ----------------------------------------------- *)
+  (*      #"neq_0_l" : #"neq" #"0" (#"1+" "n") *)
+  (* ]; *)
+  (* [:|  "n": #"natural" *)
+  (*      ----------------------------------------------- *)
+  (*      #"neq_0_r" : #"neq" (#"1+" "n") #"0" *)
+  (* ]; *)
+  (* [:|  "n": #"natural", "m": #"natural", *)
+  (*      "p" : #"neq" "n" "m" *)
+  (*      ----------------------------------------------- *)
+  (*      #"neq_1+" "p" : #"neq" (#"1+" "n") (#"1+" "m") *)
+  (* ] *)
+  ]}.
+
+
+Derive nat_lang
+       SuchThat (elab_lang_ext [] nat_lang_def nat_lang)
+       As nat_lang_wf.
+Proof. auto_elab. Qed.
+#[export] Hint Resolve nat_lang_wf : elab_pfs.
+
+
+
